Proof of trace_of

SemanticsSafetyLike.v
@@ -256,6 +256,19 @@ CoFixpoint trace_of (c:cfg) : trace.
   - exact (tcons e (trace_of c')).
 Defined.
 
+
+(* cf CPDT *)
+Definition frob (t :trace) : trace :=
+  match t with
+  | tstop => tstop
+  | tsilent => tsilent
+  | tcons e' t' => tcons e' t'
+  end.
+
+Theorem frob_eq : forall t, t = frob t.
+  destruct t; reflexivity.
+Qed.
+
 (* The usual hack to unfold CoFixpoints, but it ain't pretty and
    it still doesn't compute because of all the axioms
    TODO: update this
@@ -309,8 +322,47 @@ Lemma trace_of_eta' : forall c,
       else tcons e (trace_of c')
     end.
 Proof.
-  (* Have no idea how to prove this... *)
-Admitted.
+  intros.
+  rewrite (frob_eq (trace_of c)). simpl.
+  destruct (match classicT (stuck c) with
+  | left _ => tstop
+  | right H =>
+      let (e, H1) :=
+        indefinite_description event (fun n : event => exists n0 : cfg, ~ ~ step c n n0)
+          (Morphisms.subrelation_proper Morphisms_Prop.ex_iff_morphism tt
+             (Morphisms.subrelation_respectful
+                (Morphisms.subrelation_refl (Morphisms.pointwise_relation event iff))
+                Morphisms.iff_impl_subrelation) (fun n : event => ~ (forall c' : cfg, ~ step c n c'))
+             (fun n : event => exists n0 : cfg, ~ ~ step c n n0)
+             (fun n : event => not_forall_ex_not cfg (fun n0 : cfg => ~ step c n n0))
+             (Morphisms.iff_impl_subrelation (~ (forall (n : event) (c' : cfg), ~ step c n c'))
+                (exists n : event, ~ (forall c' : cfg, ~ step c n c'))
+                (not_forall_ex_not event (fun n : event => forall c' : cfg, ~ step c n c')) H)) in
+      let (c', _) := indefinite_description cfg (fun n : cfg => ~ ~ step c e n) H1 in
+      if classicT (silent e)
+      then
+       match classicT (can_loop_silent c') with
+       | left _ => tsilent
+       | right Hc =>
+           match not_can_loop_silent c' Hc with
+           | left Hc1 =>
+               let (e', Hc3) :=
+                 indefinite_description event (fun e0 : event => exists c'0 : cfg, steps' c' [e0] c'0)
+                   Hc1 in
+               let (c'', _) := indefinite_description cfg (fun c'0 : cfg => steps' c' [e'] c'0) Hc3 in
+               tcons e' (trace_of c'')
+           | right Hc1 =>
+               let (c'', a) :=
+                 indefinite_description cfg (fun c'0 : cfg => steps' c' [] c'0 /\ stuck c'0) Hc1 in
+               match a with
+               | conj _ _ => tstop
+               end
+           end
+       end
+      else tcons e (trace_of c')
+  end); reflexivity.
+Qed.
+
 
 (* CoFixpoint sem'_trace_of (c:cfg) : sem'' c (trace_of c). *)
 (*   rewrite trace_of_eta. destruct (classicT (stuck c)) as [H | H]. *)
